

Questions rapides 1

$$\text{A) } \frac{3}{7} + \frac{7}{21}$$

$$\text{B) } \frac{5}{6} - \frac{6}{8}$$

Correction :

$$\text{A) } \frac{3}{7} + \frac{7}{21} = \frac{9}{21} + \frac{7}{21} = \frac{16}{21}$$

$$\text{B) } \frac{5}{6} - \frac{6}{8} = \frac{5 \times 8}{6 \times 8} - \frac{6 \times 6}{6 \times 8} = \frac{4}{48}$$

Questions rapides 2

$$\text{A) } \frac{1}{4} + \frac{4}{12}$$

$$\text{B) } \frac{5}{6} - \frac{4}{8}$$

Correction :

$$\text{A) } \frac{1}{4} + \frac{4}{12} = \frac{3}{12} + \frac{4}{12} = \frac{7}{12}$$

$$\text{B) } \frac{5}{6} - \frac{4}{8} = \frac{5 \times 8}{6 \times 8} - \frac{4 \times 6}{6 \times 8} = \frac{16}{48}$$

Questions rapides 3

$$\text{A) } \frac{1}{9} + \frac{21}{27}$$

$$\text{B) } \frac{2}{3} - \frac{2}{4}$$

Correction :

$$\text{A) } \frac{1}{9} + \frac{21}{27} = \frac{3}{27} + \frac{21}{27} = \frac{24}{27}$$

$$\text{B) } \frac{2}{3} - \frac{2}{4} = \frac{2 \times 4}{3 \times 4} - \frac{2 \times 3}{3 \times 4} = \frac{2}{12}$$

Questions rapides 4

$$\text{A)} \quad \frac{3}{6} + \frac{6}{18}$$

$$\text{B)} \quad \frac{8}{9} - \frac{2}{5}$$

Correction :

$$\text{A)} \quad \frac{3}{6} + \frac{6}{18} = \frac{9}{18} + \frac{6}{18} = \frac{15}{18}$$

$$\text{B)} \quad \frac{8}{9} - \frac{2}{5} = \frac{8 \times 5}{9 \times 5} - \frac{2 \times 9}{9 \times 5} = \frac{22}{45}$$

Questions rapides 5

$$\text{A) } \frac{1}{3} + \frac{7}{9}$$

$$\text{B) } \frac{6}{7} - \frac{3}{8}$$

Correction :

$$\text{A) } \frac{1}{3} + \frac{7}{9} = \frac{3}{9} + \frac{7}{9} = \frac{10}{9}$$

$$\text{B) } \frac{6}{7} - \frac{3}{8} = \frac{6 \times 8}{7 \times 8} - \frac{3 \times 7}{7 \times 8} = \frac{27}{56}$$

Questions rapides 6

$$\text{A) } \frac{3}{8} + \frac{22}{24}$$

$$\text{B) } \frac{4}{5} - \frac{1}{3}$$

Correction :

$$\text{A) } \frac{3}{8} + \frac{22}{24} = \frac{9}{24} + \frac{22}{24} = \frac{31}{24}$$

$$\text{B) } \frac{4}{5} - \frac{1}{3} = \frac{4 \times 3}{5 \times 3} - \frac{1 \times 5}{5 \times 3} = \frac{7}{15}$$

Questions rapides 7

$$\text{A) } \frac{1}{5} + \frac{1}{15}$$

$$\text{B) } \frac{4}{5} - \frac{2}{3}$$

Correction :

$$\text{A) } \frac{1}{5} + \frac{1}{15} = \frac{3}{15} + \frac{1}{15} = \frac{4}{15}$$

$$\text{B) } \frac{4}{5} - \frac{2}{3} = \frac{4 \times 3}{5 \times 3} - \frac{2 \times 5}{5 \times 3} = \frac{2}{15}$$

Questions rapides 8

$$\text{A)} \quad \frac{1}{2} + \frac{4}{6}$$

$$\text{B)} \quad \frac{7}{8} - \frac{6}{7}$$

Correction :

$$\text{A)} \quad \frac{1}{2} + \frac{4}{6} = \frac{3}{6} + \frac{4}{6} = \frac{7}{6}$$

$$\text{B)} \quad \frac{7}{8} - \frac{6}{7} = \frac{7 \times 7}{8 \times 7} - \frac{6 \times 8}{8 \times 7} = \frac{1}{56}$$

Questions rapides 9

$$\text{A) } \frac{5}{7} + \frac{15}{21}$$

$$\text{B) } \frac{4}{6} - \frac{5}{9}$$

Correction :

$$\text{A) } \frac{5}{7} + \frac{15}{21} = \frac{15}{21} + \frac{15}{21} = \frac{30}{21}$$

$$\text{B) } \frac{4}{6} - \frac{5}{9} = \frac{4 \times 3}{6 \times 3} - \frac{5 \times 2}{6 \times 3} = \frac{12}{18} - \frac{10}{18} = \frac{2}{18} = \frac{1}{9}$$

Questions rapides 10

$$\text{A) } \frac{1}{4} + \frac{5}{12}$$

$$\text{B) } \frac{2}{4} - \frac{1}{5}$$

Correction :

$$\text{A) } \frac{1}{4} + \frac{5}{12} = \frac{3}{12} + \frac{5}{12} = \frac{8}{12}$$

$$\text{B) } \frac{2}{4} - \frac{1}{5} = \frac{2 \times 5}{4 \times 5} - \frac{1 \times 4}{4 \times 5} = \frac{6}{20}$$

Questions rapides 11

$$\text{A) } \frac{8}{9} + \frac{8}{27}$$

$$\text{B) } \frac{4}{7} - \frac{5}{9}$$

Correction :

$$\text{A) } \frac{8}{9} + \frac{8}{27} = \frac{24}{27} + \frac{8}{27} = \frac{32}{27}$$

$$\text{B) } \frac{4}{7} - \frac{5}{9} = \frac{4 \times 9}{7 \times 9} - \frac{5 \times 7}{7 \times 9} = \frac{1}{63}$$

Questions rapides 12

$$\text{A) } \frac{5}{6} + \frac{8}{18}$$

$$\text{B) } \frac{6}{9} - \frac{3}{7}$$

Correction :

$$\text{A) } \frac{5}{6} + \frac{8}{18} = \frac{15}{18} + \frac{8}{18} = \frac{23}{18}$$

$$\text{B) } \frac{6}{9} - \frac{3}{7} = \frac{6 \times 7}{9 \times 7} - \frac{3 \times 9}{9 \times 7} = \frac{15}{63}$$

Questions rapides 13

$$\text{A) } \frac{2}{3} + \frac{8}{9}$$

$$\text{B) } \frac{2}{4} - \frac{1}{5}$$

Correction :

$$\text{A) } \frac{2}{3} + \frac{8}{9} = \frac{6}{9} + \frac{8}{9} = \frac{14}{9}$$

$$\text{B) } \frac{2}{4} - \frac{1}{5} = \frac{2 \times 5}{4 \times 5} - \frac{1 \times 4}{4 \times 5} = \frac{6}{20}$$

Questions rapides 14

$$\text{A) } \frac{3}{8} + \frac{22}{24}$$

$$\text{B) } \frac{5}{6} - \frac{1}{4}$$

Correction :

$$\text{A) } \frac{3}{8} + \frac{22}{24} = \frac{9}{24} + \frac{22}{24} = \frac{31}{24}$$

$$\text{B) } \frac{5}{6} - \frac{1}{4} = \frac{5 \times 4}{6 \times 4} - \frac{1 \times 6}{6 \times 4} = \frac{14}{24}$$

Questions rapides 15

$$\text{A) } \frac{4}{5} + \frac{6}{15}$$

$$\text{B) } \frac{8}{9} - \frac{1}{8}$$

Correction :

$$\text{A) } \frac{4}{5} + \frac{6}{15} = \frac{12}{15} + \frac{6}{15} = \frac{18}{15}$$

$$\text{B) } \frac{8}{9} - \frac{1}{8} = \frac{8 \times 8}{9 \times 8} - \frac{1 \times 9}{9 \times 8} = \frac{55}{72}$$

Questions rapides 16

$$\text{A)} \quad \frac{1}{2} + \frac{5}{6}$$

$$\text{B)} \quad \frac{2}{5} - \frac{1}{4}$$

Correction :

$$\text{A)} \quad \frac{1}{2} + \frac{5}{6} = \frac{3}{6} + \frac{5}{6} = \frac{8}{6}$$

$$\text{B)} \quad \frac{2}{5} - \frac{1}{4} = \frac{2 \times 4}{5 \times 4} - \frac{1 \times 5}{5 \times 4} = \frac{3}{20}$$

Questions rapides 17

$$\text{A) } \frac{2}{7} + \frac{15}{28}$$

$$\text{B) } \frac{3}{6} - \frac{2}{4}$$

Correction :

$$\text{A) } \frac{2}{7} + \frac{15}{28} = \frac{8}{28} + \frac{15}{28} = \frac{23}{28}$$

$$\text{B) } \frac{3}{6} - \frac{2}{4} = \frac{3 \times 4}{6 \times 4} - \frac{2 \times 6}{6 \times 4} = \frac{0}{24}$$

Questions rapides 18

$$\text{A) } \frac{3}{4} + \frac{12}{16}$$

$$\text{B) } \frac{6}{8} - \frac{2}{9}$$

Correction :

$$\text{A) } \frac{3}{4} + \frac{12}{16} = \frac{12}{16} + \frac{12}{16} = \frac{24}{16}$$

$$\text{B) } \frac{6}{8} - \frac{2}{9} = \frac{6 \times 9}{8 \times 9} - \frac{2 \times 8}{8 \times 9} = \frac{38}{72}$$

Questions rapides 19

$$\text{A) } \frac{7}{9} + \frac{23}{36}$$

$$\text{B) } \frac{2}{3} - \frac{1}{6}$$

Correction :

$$\text{A) } \frac{7}{9} + \frac{23}{36} = \frac{28}{36} + \frac{23}{36} = \frac{51}{36}$$

$$\text{B) } \frac{2}{3} - \frac{1}{6} = \frac{2 \times 6}{3 \times 6} - \frac{1 \times 3}{3 \times 6} = \frac{9}{18}$$

Questions rapides 20

$$\text{A) } \frac{2}{6} + \frac{20}{24}$$

$$\text{B) } \frac{3}{6} - \frac{2}{4}$$

Correction :

$$\text{A) } \frac{2}{6} + \frac{20}{24} = \frac{8}{24} + \frac{20}{24} = \frac{28}{24}$$

$$\text{B) } \frac{3}{6} - \frac{2}{4} = \frac{3 \times 4}{6 \times 4} - \frac{2 \times 6}{6 \times 4} = \frac{0}{24}$$

Questions rapides 21

$$\text{A) } \frac{1}{3} + \frac{4}{12}$$

$$\text{B) } \frac{8}{9} - \frac{5}{8}$$

Correction :

$$\text{A) } \frac{1}{3} + \frac{4}{12} = \frac{4}{12} + \frac{4}{12} = \frac{8}{12}$$

$$\text{B) } \frac{8}{9} - \frac{5}{8} = \frac{8 \times 8}{9 \times 8} - \frac{5 \times 9}{9 \times 8} = \frac{19}{72}$$

Questions rapides 22

$$\text{A) } \frac{3}{8} + \frac{31}{32}$$

$$\text{B) } \frac{1}{3} - \frac{1}{7}$$

Correction :

$$\text{A) } \frac{3}{8} + \frac{31}{32} = \frac{12}{32} + \frac{31}{32} = \frac{43}{32}$$

$$\text{B) } \frac{1}{3} - \frac{1}{7} = \frac{1 \times 7}{3 \times 7} - \frac{1 \times 3}{3 \times 7} = \frac{4}{21}$$

Questions rapides 23



$$\text{A)} \quad \frac{3}{5} + \frac{11}{20}$$

$$\text{B)} \quad \frac{4}{5} - \frac{2}{6}$$

Correction :

$$\text{A)} \quad \frac{3}{5} + \frac{11}{20} = \frac{12}{20} + \frac{11}{20} = \frac{23}{20}$$

$$\text{B)} \quad \frac{4}{5} - \frac{2}{6} = \frac{4 \times 6}{5 \times 6} - \frac{2 \times 5}{5 \times 6} = \frac{14}{30}$$

Questions rapides 24

$$\text{A) } \frac{1}{2} + \frac{3}{8}$$

$$\text{B) } \frac{5}{8} - \frac{1}{3}$$

Correction :

$$\text{A) } \frac{1}{2} + \frac{3}{8} = \frac{4}{8} + \frac{3}{8} = \frac{7}{8}$$

$$\text{B) } \frac{5}{8} - \frac{1}{3} = \frac{5 \times 3}{8 \times 3} - \frac{1 \times 8}{8 \times 3} = \frac{7}{24}$$

Questions rapides 25

$$\text{A) } \frac{5}{7} + \frac{2}{28}$$

$$\text{B) } \frac{7}{8} - \frac{1}{3}$$

Correction :

$$\text{A) } \frac{5}{7} + \frac{2}{28} = \frac{20}{28} + \frac{2}{28} = \frac{22}{28}$$

$$\text{B) } \frac{7}{8} - \frac{1}{3} = \frac{7 \times 3}{8 \times 3} - \frac{1 \times 8}{8 \times 3} = \frac{13}{24}$$

Questions rapides 26

$$\text{A) } \frac{3}{4} + \frac{8}{16}$$

$$\text{B) } \frac{5}{6} - \frac{1}{5}$$

Correction :

$$\text{A) } \frac{3}{4} + \frac{8}{16} = \frac{12}{16} + \frac{8}{16} = \frac{20}{16}$$

$$\text{B) } \frac{5}{6} - \frac{1}{5} = \frac{5 \times 5}{6 \times 5} - \frac{1 \times 6}{6 \times 5} = \frac{19}{30}$$

Questions rapides 27

$$\text{A) } \frac{7}{9} + \frac{14}{36}$$

$$\text{B) } \frac{2}{4} - \frac{1}{7}$$

Correction :

$$\text{A) } \frac{7}{9} + \frac{14}{36} = \frac{28}{36} + \frac{14}{36} = \frac{42}{36}$$

$$\text{B) } \frac{2}{4} - \frac{1}{7} = \frac{2 \times 7}{4 \times 7} - \frac{1 \times 4}{4 \times 7} = \frac{10}{28}$$

Questions rapides 28



$$\text{A) } \frac{4}{6} + \frac{20}{24}$$

$$\text{B) } \frac{6}{9} - \frac{4}{10}$$

Correction :

$$\text{A) } \frac{4}{6} + \frac{20}{24} = \frac{16}{24} + \frac{20}{24} = \frac{36}{24}$$

$$\text{B) } \frac{6}{9} - \frac{4}{10} = \frac{6 \times 10}{9 \times 10} - \frac{4 \times 9}{9 \times 10} = \frac{24}{90}$$

Questions rapides 29

$$\text{A) } \frac{2}{3} + \frac{4}{12}$$

$$\text{B) } \frac{4}{7} - \frac{2}{5}$$

Correction :

$$\text{A) } \frac{2}{3} + \frac{4}{12} = \frac{8}{12} + \frac{4}{12} = \frac{12}{12}$$

$$\text{B) } \frac{4}{7} - \frac{2}{5} = \frac{4 \times 5}{7 \times 5} - \frac{2 \times 7}{7 \times 5} = \frac{6}{35}$$

Questions rapides 30

$$\text{A) } \frac{3}{8} + \frac{6}{32}$$

$$\text{B) } \frac{4}{5} - \frac{5}{7}$$

Correction :

$$\text{A) } \frac{3}{8} + \frac{6}{32} = \frac{12}{32} + \frac{6}{32} = \frac{18}{32}$$

$$\text{B) } \frac{4}{5} - \frac{5}{7} = \frac{4 \times 7}{5 \times 7} - \frac{5 \times 5}{5 \times 7} = \frac{3}{35}$$

Questions rapides 31

$$\text{A) } \frac{2}{5} + \frac{1}{20}$$

$$\text{B) } \frac{7}{9} - \frac{2}{4}$$

Correction :

$$\text{A) } \frac{2}{5} + \frac{1}{20} = \frac{8}{20} + \frac{1}{20} = \frac{9}{20}$$

$$\text{B) } \frac{7}{9} - \frac{2}{4} = \frac{7 \times 4}{9 \times 4} - \frac{2 \times 9}{9 \times 4} = \frac{10}{36}$$

Questions rapides 32

$$\text{A) } \frac{1}{2} + \frac{2}{8}$$

$$\text{B) } \frac{3}{4} - \frac{4}{7}$$

Correction :

$$\text{A) } \frac{1}{2} + \frac{2}{8} = \frac{4}{8} + \frac{2}{8} = \frac{6}{8}$$

$$\text{B) } \frac{3}{4} - \frac{4}{7} = \frac{3 \times 7}{4 \times 7} - \frac{4 \times 4}{4 \times 7} = \frac{5}{28}$$

Questions rapides 33



$$\text{A) } \frac{2}{7} + \frac{9}{14}$$

$$\text{B) } \frac{3}{6} - \frac{2}{5}$$

Correction :

$$\text{A) } \frac{2}{7} + \frac{9}{14} = \frac{4}{14} + \frac{9}{14} = \frac{13}{14}$$

$$\text{B) } \frac{3}{6} - \frac{2}{5} = \frac{3 \times 5}{6 \times 5} - \frac{2 \times 6}{6 \times 5} = \frac{3}{30}$$

Questions rapides 34

$$\text{A) } \frac{3}{4} + \frac{6}{8}$$

$$\text{B) } \frac{2}{4} - \frac{1}{9}$$

Correction :

$$\text{A) } \frac{3}{4} + \frac{6}{8} = \frac{6}{8} + \frac{6}{8} = \frac{12}{8}$$

$$\text{B) } \frac{2}{4} - \frac{1}{9} = \frac{2 \times 9}{4 \times 9} - \frac{1 \times 4}{4 \times 9} = \frac{14}{36}$$

Questions rapides 35



$$\text{A) } \frac{6}{9} + \frac{8}{18}$$

$$\text{B) } \frac{6}{8} - \frac{2}{4}$$

Correction :

$$\text{A) } \frac{6}{9} + \frac{8}{18} = \frac{12}{18} + \frac{8}{18} = \frac{20}{18}$$

$$\text{B) } \frac{6}{8} - \frac{2}{4} = \frac{6 \times 4}{8 \times 4} - \frac{2 \times 8}{8 \times 4} = \frac{8}{32}$$

Questions rapides 36



$$\text{A) } \frac{4}{6} + \frac{8}{12}$$

$$\text{B) } \frac{1}{6} - \frac{1}{7}$$

Correction :

$$\text{A) } \frac{4}{6} + \frac{8}{12} = \frac{8}{12} + \frac{8}{12} = \frac{16}{12}$$

$$\text{B) } \frac{1}{6} - \frac{1}{7} = \frac{1 \times 7}{6 \times 7} - \frac{1 \times 6}{6 \times 7} = \frac{1}{42}$$

Questions rapides 37

$$\text{A)} \quad \frac{1}{3} + \frac{2}{6}$$

$$\text{B)} \quad \frac{1}{5} - \frac{1}{8}$$

Correction :

$$\text{A)} \quad \frac{1}{3} + \frac{2}{6} = \frac{2}{6} + \frac{2}{6} = \frac{4}{6}$$

$$\text{B)} \quad \frac{1}{5} - \frac{1}{8} = \frac{1 \times 8}{5 \times 8} - \frac{1 \times 5}{5 \times 8} = \frac{3}{40}$$

Questions rapides 38



$$\text{A) } \frac{3}{8} + \frac{13}{16}$$

$$\text{B) } \frac{7}{9} - \frac{1}{3}$$

Correction :

$$\text{A) } \frac{3}{8} + \frac{13}{16} = \frac{6}{16} + \frac{13}{16} = \frac{19}{16}$$

$$\text{B) } \frac{7}{9} - \frac{1}{3} = \frac{7 \times 3}{9 \times 3} - \frac{1 \times 3}{3 \times 3} = \frac{21}{27} - \frac{3}{27} = \frac{18}{27} = \frac{2}{3}$$

Questions rapides 39



$$\text{A) } \frac{1}{5} + \frac{7}{10}$$

$$\text{B) } \frac{1}{6} - \frac{1}{7}$$

Correction :

$$\text{A) } \frac{1}{5} + \frac{7}{10} = \frac{2}{10} + \frac{7}{10} = \frac{9}{10}$$

$$\text{B) } \frac{1}{6} - \frac{1}{7} = \frac{1 \times 7}{6 \times 7} - \frac{1 \times 6}{6 \times 7} = \frac{1}{42}$$

Questions rapides 40

$$\text{A) } \frac{1}{2} + \frac{1}{4}$$

$$\text{B) } \frac{7}{8} - \frac{3}{5}$$

Correction :

$$\text{A) } \frac{1}{2} + \frac{1}{4} = \frac{2}{4} + \frac{1}{4} = \frac{3}{4}$$

$$\text{B) } \frac{7}{8} - \frac{3}{5} = \frac{7 \times 5}{8 \times 5} - \frac{3 \times 8}{8 \times 5} = \frac{11}{40}$$

Questions rapides 41

$$\text{A) } \frac{5}{7} + \frac{6}{14}$$

$$\text{B) } \frac{2}{3} - \frac{2}{4}$$

Correction :

$$\text{A) } \frac{5}{7} + \frac{6}{14} = \frac{10}{14} + \frac{6}{14} = \frac{16}{14}$$

$$\text{B) } \frac{2}{3} - \frac{2}{4} = \frac{2 \times 4}{3 \times 4} - \frac{2 \times 3}{3 \times 4} = \frac{2}{12}$$

Questions rapides 42



$$\text{A) } \frac{3}{4} + \frac{5}{8}$$

$$\text{B) } \frac{7}{8} - \frac{1}{5}$$

Correction :

$$\text{A) } \frac{3}{4} + \frac{5}{8} = \frac{6}{8} + \frac{5}{8} = \frac{11}{8}$$

$$\text{B) } \frac{7}{8} - \frac{1}{5} = \frac{7 \times 5}{8 \times 5} - \frac{1 \times 8}{8 \times 5} = \frac{27}{40}$$

Questions rapides 43



$$\text{A) } \frac{5}{9} + \frac{10}{18}$$

$$\text{B) } \frac{7}{8} - \frac{1}{6}$$

Correction :

$$\text{A) } \frac{5}{9} + \frac{10}{18} = \frac{10}{18} + \frac{10}{18} = \frac{20}{18}$$

$$\text{B) } \frac{7}{8} - \frac{1}{6} = \frac{7 \times 6}{8 \times 6} - \frac{1 \times 8}{8 \times 6} = \frac{34}{48}$$

Questions rapides 44

$$\text{A)} \quad \frac{1}{6} + \frac{8}{12}$$

$$\text{B)} \quad \frac{3}{4} - \frac{2}{3}$$

Correction :

$$\text{A)} \quad \frac{1}{6} + \frac{8}{12} = \frac{2}{12} + \frac{8}{12} = \frac{10}{12}$$

$$\text{B)} \quad \frac{3}{4} - \frac{2}{3} = \frac{3 \times 3}{4 \times 3} - \frac{2 \times 4}{4 \times 3} = \frac{1}{12}$$

Questions rapides 45

$$\text{A) } \frac{1}{3} + \frac{3}{6}$$

$$\text{B) } \frac{4}{9} - \frac{2}{5}$$

Correction :

$$\text{A) } \frac{1}{3} + \frac{3}{6} = \frac{2}{6} + \frac{3}{6} = \frac{5}{6}$$

$$\text{B) } \frac{4}{9} - \frac{2}{5} = \frac{4 \times 5}{9 \times 5} - \frac{2 \times 9}{9 \times 5} = \frac{2}{45}$$

Questions rapides 46



$$\text{A)} \quad \frac{3}{8} + \frac{9}{16}$$

$$\text{B)} \quad \frac{3}{8} - \frac{1}{7}$$

Correction :

$$\text{A)} \quad \frac{3}{8} + \frac{9}{16} = \frac{6}{16} + \frac{9}{16} = \frac{15}{16}$$

$$\text{B)} \quad \frac{3}{8} - \frac{1}{7} = \frac{3 \times 7}{8 \times 7} - \frac{1 \times 8}{8 \times 7} = \frac{13}{56}$$

Questions rapides 47

$$\text{A) } \frac{4}{5} + \frac{3}{10}$$

$$\text{B) } \frac{4}{5} - \frac{7}{9}$$

Correction :

$$\text{A) } \frac{4}{5} + \frac{3}{10} = \frac{8}{10} + \frac{3}{10} = \frac{11}{10}$$

$$\text{B) } \frac{4}{5} - \frac{7}{9} = \frac{4 \times 9}{5 \times 9} - \frac{7 \times 5}{5 \times 9} = \frac{1}{45}$$

Questions rapides 48



$$\text{A) } \frac{1}{2} + \frac{3}{4}$$

$$\text{B) } \frac{4}{5} - \frac{2}{9}$$

Correction :

$$\text{A) } \frac{1}{2} + \frac{3}{4} = \frac{2}{4} + \frac{3}{4} = \frac{5}{4}$$

$$\text{B) } \frac{4}{5} - \frac{2}{9} = \frac{4 \times 9}{5 \times 9} - \frac{2 \times 5}{5 \times 9} = \frac{26}{45}$$

Questions rapides 49

$$\text{A) } \frac{2}{7} + \frac{7}{21}$$

$$\text{B) } \frac{6}{7} - \frac{1}{8}$$

Correction :

$$\text{A) } \frac{2}{7} + \frac{7}{21} = \frac{6}{21} + \frac{7}{21} = \frac{13}{21}$$

$$\text{B) } \frac{6}{7} - \frac{1}{8} = \frac{6 \times 8}{7 \times 8} - \frac{1 \times 7}{7 \times 8} = \frac{41}{56}$$

Questions rapides 50

$$\text{A)} \quad \frac{3}{4} + \frac{6}{12}$$

$$\text{B)} \quad \frac{2}{5} - \frac{1}{9}$$

Correction :

$$\text{A)} \quad \frac{3}{4} + \frac{6}{12} = \frac{9}{12} + \frac{6}{12} = \frac{15}{12}$$

$$\text{B)} \quad \frac{2}{5} - \frac{1}{9} = \frac{2 \times 9}{5 \times 9} - \frac{1 \times 5}{5 \times 9} = \frac{13}{45}$$